Addition32 spec in terms of UInt32

Clean/Gadgets/Addition32/Addition32.lean
@@ -2,6 +2,7 @@ import Clean.Gadgets.Addition32.Addition32Full
 import Clean.Types.U32
 import Clean.Gadgets.Addition32.Theorems
 import Clean.Utils.Primes
+import Clean.Circuit.StructuralLemmas
 
 namespace Gadgets.Addition32
 variable {p : ℕ} [Fact p.Prime] [Fact (p > 512)]
@@ -55,3 +56,56 @@ def circuit : FormalCircuit (F p) Inputs U32 where
   soundness
   completeness
 end Gadgets.Addition32
+lemma UInt32.ofNat.inj_on_small (a b : ℕ) (h_a : a < UInt32.size) (h_b : b < UInt32.size) :
+    UInt32.ofNat a = UInt32.ofNat b →
+    a = b := by
+  intro h
+  rw[← UInt32.toNat_ofNat_of_lt' (n := a), ← UInt32.toNat_ofNat_of_lt' (n := b), h]
+  · assumption
+  · assumption
+
+lemma UInt32.ofNat.injEq_on_small (a b : ℕ) (h_a : a < UInt32.size) (h_b : b < UInt32.size) :
+    UInt32.ofNat a = UInt32.ofNat b ↔
+    a = b := by
+  constructor
+  · apply UInt32.ofNat.inj_on_small
+    · assumption
+    · assumption
+  · intro h
+    rw [h]
+
+-- A version of Gadgets.Addition32 whose specification is written in terms of UInt32
+namespace Gadgets.Addition32.UInt32
+  variable {p : ℕ} [Fact p.Prime] [Fact (p > 512)]
+
+  omit [Fact (Nat.Prime p)] [Fact (p > 512)] in
+  lemma U32_value_rawValueU32_bridge (a b c : U32 (F p)) (h_a : a.Normalized) :
+      a.value = (b.value + c.value) % 2 ^ 32 ↔
+      a.rawValueU32 = b.rawValueU32 + c.rawValueU32 := by
+    simp only [U32.rawValueU32]
+    constructor
+    · intro h
+      simp only [h]
+      rw [UInt32.ofNat_mod_size]
+      simp only [UInt32.ofNat_add]
+    · intro h
+      rw[← UInt32.toNat_ofNat_of_lt' (n := a.value), h]
+      · symm
+        rw[← UInt32.ofNat_eq_iff_mod_eq_toNat]
+        rw[← UInt32.ofNat_add]
+      · apply U32.value_lt_of_normalized; assumption
+
+  def Spec (input: Gadgets.Addition32.Inputs (F p)) (z : U32 (F p)) :=
+    let ⟨x, y⟩ := input
+    z.rawValueU32 = x.rawValueU32 + y.rawValueU32 ∧ z.Normalized
+  def circuit :=
+    Gadgets.Addition32.circuit (p := p).weakenSpec Spec (by
+      intro input output
+      simp only[Gadgets.Addition32.circuit]
+      simp only[Assumptions, Addition32.Spec, Spec]
+      intro h_normalized h_spec
+      rw [← U32_value_rawValueU32_bridge] <;> tauto
+    )
+  lemma circuit_Assumptions :
+    circuit (p := p).Assumptions = Assumptions := by rfl
+end Gadgets.Addition32.UInt32
